workloads/Coq/IFCProplang/Src/Machine.v
@@ -44,9 +44,9 @@ Definition default_table : table := fun op =>
 (* ---"OpLab"--- *)
 
 (*! *)
-(* | OpLab => ≪ TRUE , BOT , LabPC ≫ *)
+| OpLab => ≪ TRUE , BOT , LabPC ≫
 (*!! OpLab_1 *)
- | OpLab => ≪ TRUE , BOT , BOT ≫
+ (* | OpLab => ≪ TRUE , BOT , BOT ≫ *)
 
 (* ---"OpMLab"--- *)
 
