workloads/Coq/IFCProplang/Strategies/VariationalFuzzer.v
@@ -80,7 +80,7 @@ Definition mutate_variation (v: @Variation SState) : G (@Variation SState) :=
   let '(St im m s r pc) := st1 in
   bindGen (mutate_instructions im st1 l) (fun im' =>
   returnGen (Var l (St im' m s r pc) st2)).
-
+(* 
 Definition test_propEENI :=
   @targetLoop 
     number_of_trials 
@@ -103,6 +103,76 @@ Definition test_propEENI :=
     (HeapSeedPool.(mkPool) tt) 
     HillClimbingUtility.
 
-Sample test_propEENI.
+     *)
+
+    
+
+
+
+Fixpoint low_indist (fuel: nat) (t: table) (v: Variation) :=
+  match fuel with
+  | 0 => true
+  | S n' =>
+    let '(Var lab st1 st2) := v in
+    let next_step : option ((option SState) * (option SState)) := 
+      match is_low_SState st1 lab, is_low_SState st2 lab with
+      | true, true => 
+        (* When both states are low, we check indistinguishability *)
+        if indist lab st1 st2 then
+          (* If they are indistinguishable, we step forward *)
+          Some (fstep t st1, fstep t st2)
+          (* If they are distinguishable, we found a bug *)
+        else None
+      | true, false => 
+        (* If one of the states is low, we step the other *)
+        Some (fstep t st1, Some st2)
+      | false, true =>
+        (* If one of the states is low, we step the other *)
+        Some (Some st1, fstep t st2)
+      | false, false =>
+        (* If both states are high, we step both *)
+        Some (fstep t st1, fstep t st2)
+      end in
+    match next_step with
+    | None => 
+      (* Two low states were distinguishable *)
+      false
+    | Some (Some st1', Some st2') =>
+      (* Both states stepped, we continue *)
+      low_indist n' t (Var lab st1' st2')
+    | _ =>
+      (* One of the traces ended, so we stop *)
+      true
+    end
+  end.
+
+Definition propLLNI :=
+  ForAll "v" (fun _ => gen_variation_SState) (fun _ _ => gen_variation_SState) (fun _ => shrink) (fun _ => show) (
+  Implies ((@Variation SState) · ∅) (fun '((Var lab st1 st2), _) => indist lab st1 st2) (
+  Implies ((@Variation SState) · ∅) (fun '((Var lab st1 st2), _) => well_formed st1) (
+  Implies ((@Variation SState) · ∅) (fun '((Var lab st1 st2), _) => well_formed st2) (
+  Check ((@Variation SState) · ∅) (fun '(Var lab st1 st2, _) => 
+    low_indist 1000 default_table (Var lab st1 st2)
+  ))))).
+
+
+Definition fuzzPropLLNI :=
+  fuzzLoop num_tests propLLNI
+  (HeapSeedPool.(mkPool) tt) HillClimbingUtility
+.
+Check HeapSeedPool.(mkPool) tt.
+Check LeftistHeap.Heap.
+
+Check propLLNI.
+Check HillClimbingUtility.
+Check (fun _ => 10%Z).
+Definition test_propLLNI :=
+  targetLoop 
+    10000 
+    propLLNI
+    (fun _ => 10%Z).
+
+Check test_propLLNI.
+
   
 (*! QuickProp test_propEENI. *)
